Progress in proof of [dll_insert_at_tail] iface impl

ind/DoublyLinkedListIface.fst
@@ -359,22 +359,16 @@ let dll_insert_at_head #t d n =
 #set-options "--z3rlimit 40 --max_fuel 2 --max_ifuel 1"
 
 let dll_insert_at_tail #t d n =
-  let h00 = HST.get () in // temp
   HST.push_frame ();
   let h0 = HST.get () in
   let y = DLL.dll_insert_at_tail (!*d) n in
   let h' = HST.get () in
   d *= y;
   let h1 = HST.get () in
-  HST.pop_frame ();
-  let h11 = HST.get () in // temp
-  // assert (B.modifies (fp_dll h11 d) h00 h11);
-  assume (fp_dll h11 d `loc_equiv` B.loc_union (fp_dll h00 d) (fp_node n));
-  assume (dll_valid h11 d);
-  // assert (node_valid h11 n);
-  assume (unchanged_node_vals h00 h11 (as_list h11 d));
-  // assert (as_list h11 d == l_insert_at_tail (as_list h00 d) n);
-  ()
+  assume (DLL.dll_fp0 (d@h1) `loc_equiv` B.loc_union (DLL.dll_fp0 (d@h0)) (fp_node n));
+  assume (_pred_nl_disjoint h0 (as_list h1 d));
+  _lemma_unchanged_node_vals_transitive h0 h' h1 (as_list h1 d);
+  HST.pop_frame ()
 
 #reset-options
 
